lean/Och/Std.lean
@@ -1,13 +1,11 @@
 import Och.Std.Unit
 import Och.Std.Bool
 import Och.Std.DBool
-import Och.Std.Nat
 import Och.Std.DNat
 import Och.Std.Pair
 import Och.Std.Sigma
 import Och.Std.Array
 import Och.Std.Vec
 import Och.Std.DFin
-import Och.Std.Fin
 import Och.Std.Id
 import Och.Std.Mu
